yalla/ll_smp.v
@@ -21,18 +21,12 @@ Context {atom : InfDecType}.
 (** ** 1. define formulas *)
 
 Inductive formula :=
-| var : atom -> formula
-| covar : atom -> formula
-| one : formula
-| bot : formula
-| tens : formula -> formula -> formula
-| parr : formula -> formula -> formula
-| zero : formula
-| top : formula
-| aplus : formula -> formula -> formula
-| awith : formula -> formula -> formula
-| oc : formula -> formula
-| wn : formula -> formula.
+| var (_ : atom) | covar (_ : atom)
+| one | bot
+| tens (_ _ : formula) | parr (_ _ : formula)
+| zero | top
+| aplus (_ _ : formula) | awith (_ _ : formula)
+| oc (_ : formula) | wn (_ : formula).
 
 Fixpoint dual A :=
 match A with
@@ -71,54 +65,49 @@ end.
 
 Lemma ll2ll_inj : injective ll2ll.
 Proof.
-intros A.
-induction A ; intros B Heq ;
-  destruct B ; inversion Heq ;
-  try apply IHA in H0 ;
-  try apply IHA1 in H0 ;
-  try apply IHA2 in H1 ; subst ;
-  reflexivity.
+intros A. induction A; intros B Heq;
+  destruct B; inversion Heq;
+  try apply IHA in H0; try apply IHA1 in H0; try apply IHA2 in H1; subst; reflexivity.
 Qed.
 
 Lemma ll2ll_dual A : formulas.dual (ll2ll A) = ll2ll (dual A).
 Proof. induction A; cbn; rewrite ? IHA, ? IHA1, ? IHA2; reflexivity. Qed.
 
-Lemma ll2ll_map_wn l :
-  map ll2ll (map wn l) = map formulas.wn (map ll2ll l).
-Proof. induction l; [ | cbn; rewrite IHl ]; reflexivity. Qed.
+Lemma ll2ll_map_wn l : map ll2ll (map wn l) = map formulas.wn (map ll2ll l).
+Proof. induction l as [|a l IHl]; [ | cbn; rewrite IHl ]; reflexivity. Qed.
 
 Lemma ll2ll_map_wn_inv l1 l2 : map formulas.wn l1 = map ll2ll l2 ->
-  { l2' | l2 = map wn l2' /\ l1 = map ll2ll l2' }.
+  { l2' | l2 = map wn l2' & l1 = map ll2ll l2' }.
 Proof.
 induction l1 in l2 |- *; intro Heq; destruct l2; inversion Heq.
-- exists nil; split; reflexivity.
+- exists nil; reflexivity.
 - apply IHl1 in H1.
   destruct f; inversion H0; subst.
-  destruct H1 as (l2' & Heq1 & H1); subst.
-  exists (f :: l2'); split; reflexivity.
+  destruct H1 as [l2' -> ->].
+  exists (f :: l2'); reflexivity.
 Qed.
 
 
 (** ** 3. define proofs *)
 
 Inductive ll : list formula -> Type :=
-| ax_r : forall X, ll (covar X :: var X :: nil)
-| ex_r : forall l1 l2, ll l1 -> Permutation_Type l1 l2 -> ll l2
+| ax_r X : ll (covar X :: var X :: nil)
+| ex_r l1 l2 : ll l1 -> Permutation_Type l1 l2 -> ll l2
 | one_r : ll (one :: nil)
-| bot_r : forall l, ll l -> ll (bot :: l)
-| tens_r : forall A B l1 l2, ll (A :: l1) -> ll (B :: l2) -> ll (tens A B :: l1 ++ l2)
-| parr_r : forall A B l, ll (A :: B :: l) -> ll (parr A B :: l)
-| top_r : forall l, ll (top :: l)
-| plus_r1 : forall A B l, ll (A :: l) -> ll (aplus A B :: l)
-| plus_r2 : forall A B l, ll (A :: l) -> ll (aplus B A :: l)
-| with_r : forall A B l, ll (A :: l) -> ll (B :: l) -> ll (awith A B :: l)
-| oc_r : forall A l, ll (A :: List.map wn l) -> ll (oc A :: List.map wn l)
-| de_r : forall A l, ll (A :: l) -> ll (wn A :: l)
-| wk_r : forall A l, ll l -> ll (wn A :: l)
-| co_r : forall A l, ll (wn A :: wn A :: l) -> ll (wn A :: l).
+| bot_r l : ll l -> ll (bot :: l)
+| tens_r A B l1 l2 : ll (A :: l1) -> ll (B :: l2) -> ll (tens A B :: l1 ++ l2)
+| parr_r A B l : ll (A :: B :: l) -> ll (parr A B :: l)
+| top_r l : ll (top :: l)
+| plus_r1 A B l : ll (A :: l) -> ll (aplus A B :: l)
+| plus_r2 A B l : ll (A :: l) -> ll (aplus B A :: l)
+| with_r A B l : ll (A :: l) -> ll (B :: l) -> ll (awith A B :: l)
+| oc_r A l : ll (A :: List.map wn l) -> ll (oc A :: List.map wn l)
+| de_r A l : ll (A :: l) -> ll (wn A :: l)
+| wk_r A l : ll l -> ll (wn A :: l)
+| co_r A l : ll (wn A :: wn A :: l) -> ll (wn A :: l).
 
 Instance ll_perm : Proper ((@Permutation_Type _) ==> arrow) ll.
-Proof. intros l1 l2 HP pi; eapply ex_r; eassumption. Qed.
+Proof. intros l1 l2 HP pi. eapply ex_r; eassumption. Qed.
 
 (** ** 4. characterize corresponding [ll] fragment *)
 
@@ -128,75 +117,64 @@ Proof. intros l1 l2 HP pi; eapply ex_r; eassumption. Qed.
 
 Lemma ll2llfrag l : ll l -> ll_fragments.ll_ll (map ll2ll l).
 Proof.
-intros pi; induction pi; try (now constructor); try rewrite map_app.
+intros pi. induction pi; try (constructor; assumption); rewrite ? map_app.
 - eapply ll_def.ex_r; [ eassumption | ].
-  apply Permutation_Type_map; assumption.
+  apply Permutation_Type_map. assumption.
 - eapply ll_def.ex_r.
   + apply (ll_def.tens_r IHpi1 IHpi2).
-  + list_simpl; apply Permutation_Type_cons, Permutation_Type_app_comm; reflexivity.
-- cbn; rewrite ll2ll_map_wn.
-  apply ll_def.oc_r.
-  rewrite <- ll2ll_map_wn; assumption.
+  + list_simpl. apply Permutation_Type_cons, Permutation_Type_app_comm. reflexivity.
+- cbn. rewrite ll2ll_map_wn. apply ll_def.oc_r. rewrite <- ll2ll_map_wn. assumption.
 Qed.
 
 Lemma llfrag2ll l : ll_fragments.ll_ll (map ll2ll l) -> ll l.
 Proof.
 intros pi.
 remember (map ll2ll l) as l0.
-induction pi in l, Heql0 |- *; subst; try (inversion f ; fail).
-- symmetry in Heql0; decomp_map_inf Heql0; subst.
+induction pi in l, Heql0 |- *; subst; try discriminate f.
+- symmetry in Heql0. decomp_map_inf Heql0. subst.
   destruct l2; inversion Heql4.
   destruct x; inversion Heql2.
   destruct x0; inversion Heql0.
   apply ax_r.
 - cbn in p.
-  apply Permutation_Type_map_inv in p.
-  destruct p as [l'' Heq HP].
-  apply Permutation_Type_sym in HP.
+  apply Permutation_Type_map_inv in p as [l'' Heq HP%Permutation_Type_sym].
   eapply ex_r; [ apply IHpi | ]; eassumption.
-- symmetry in Heql0; decomp_map_inf Heql0; subst; symmetry in Heql0.
-  cbn in Heql0; apply ll2ll_map_wn_inv in Heql0; destruct Heql0 as (l & ? & ?); subst.
-  apply Permutation_Type_map_inv in p as [l' Heq HP]; subst.
+- symmetry in Heql0. decomp_map_inf Heql0. subst. symmetry in Heql0.
+  cbn in Heql0. apply ll2ll_map_wn_inv in Heql0 as [l -> ->].
+  apply Permutation_Type_map_inv in p as [l' -> HP].
   eapply ex_r; [ apply IHpi; rewrite <- ll2ll_map_wn, <- ? map_app; reflexivity | ].
   symmetry in HP.
-  apply Permutation_Type_app_head, Permutation_Type_app_tail, Permutation_Type_map; assumption.
-- inversion i.
-- destruct l; inversion Heql0; destruct f; inversion H0.
-  destruct l; inversion H1.
+  apply Permutation_Type_app_head, Permutation_Type_app_tail, Permutation_Type_map. assumption.
+- destruct l; inversion Heql0. destruct f; inversion H0. destruct l; inversion H1.
   apply one_r.
-- destruct l; inversion Heql0; destruct f; inversion H0.
-  apply bot_r, IHpi; assumption.
-- symmetry in Heql0; decomp_map_inf Heql0; subst.
+- destruct l; inversion Heql0. destruct f; inversion H0.
+  apply bot_r, IHpi. assumption.
+- symmetry in Heql0. decomp_map_inf Heql0. subst.
   destruct x; inversion Heql2; subst.
   eapply ex_r; [ apply tens_r | ].
-  + apply IHpi1; reflexivity.
-  + apply IHpi2; reflexivity.
+  + apply IHpi1. reflexivity.
+  + apply IHpi2. reflexivity.
   + apply Permutation_Type_cons; [ reflexivity | apply Permutation_Type_app_comm ].
-- destruct l; inversion Heql0.
-  destruct f; inversion H0; subst.
-  apply parr_r, IHpi; reflexivity.
-- destruct l; inversion Heql0; destruct f; inversion H0.
+- destruct l; inversion Heql0. destruct f; inversion H0. subst.
+  apply parr_r, IHpi. reflexivity.
+- destruct l; inversion Heql0. destruct f; inversion H0.
   apply top_r.
-- destruct l; inversion Heql0; destruct f; inversion H0; subst.
-  apply plus_r1, IHpi; reflexivity.
-- destruct l; inversion Heql0; destruct f; inversion H0; subst.
-  apply plus_r2, IHpi; reflexivity.
-- destruct l; inversion Heql0; destruct f; inversion H0; subst.
+- destruct l; inversion Heql0. destruct f; inversion H0. subst.
+  apply plus_r1, IHpi. reflexivity.
+- destruct l; inversion Heql0. destruct f; inversion H0. subst.
+  apply plus_r2, IHpi. reflexivity.
+- destruct l; inversion Heql0. destruct f; inversion H0. subst.
   apply with_r; [ apply IHpi1 | apply IHpi2 ]; reflexivity.
-- destruct l; inversion Heql0.
-  destruct f; inversion H0; subst.
-  apply ll2ll_map_wn_inv in H1 as (l'' & -> & ->).
+- destruct l; inversion Heql0. destruct f; inversion H0. subst.
+  apply ll2ll_map_wn_inv in H1 as [l'' -> ->].
   apply oc_r, IHpi.
-  cbn ; rewrite ll2ll_map_wn; reflexivity.
-- destruct l; inversion Heql0.
-  destruct f ; inversion H0 ; subst.
-  apply de_r, IHpi; reflexivity.
-- destruct l; inversion Heql0.
-  destruct f; inversion H0; subst.
-  apply wk_r, IHpi; reflexivity.
-- destruct l; inversion Heql0.
-  destruct f; inversion H0; subst.
-  apply co_r, IHpi; reflexivity.
+  cbn. rewrite ll2ll_map_wn. reflexivity.
+- destruct l; inversion Heql0. destruct f ; inversion H0. subst.
+  apply de_r, IHpi. reflexivity.
+- destruct l; inversion Heql0. destruct f; inversion H0. subst.
+  apply wk_r, IHpi. reflexivity.
+- destruct l; inversion Heql0. destruct f; inversion H0. subst.
+  apply co_r, IHpi. reflexivity.
 - destruct a.
 Qed.
 
@@ -207,24 +185,20 @@ Qed.
 
 Lemma ax_gen_r A : ll (dual A :: A :: nil).
 Proof.
-apply llfrag2ll.
-cbn ; rewrite <- ll2ll_dual.
+apply llfrag2ll. cbn. rewrite <- ll2ll_dual.
 eapply ll_def.ex_r; [ apply ll_def.ax_exp | apply Permutation_Type_swap ].
 Qed.
 
 (** *** cut admissibility *)
 
-Lemma cut_r A l1 l2 :
-  ll (A :: l1) -> ll (dual A :: l2) -> ll (l1 ++ l2).
+Lemma cut_r A l1 l2 : ll (A :: l1) -> ll (dual A :: l2) -> ll (l1 ++ l2).
 Proof.
-intros pi1 pi2.
+intros pi1%ll2llfrag pi2%ll2llfrag.
 apply llfrag2ll.
-rewrite map_app.
-eapply ll_cut.cut_r_axfree.
+rewrite map_app. eapply ll_cut.cut_r_axfree.
 - intros [].
-- apply ll2llfrag in pi2.
-  cbn in pi2; rewrite <- ll2ll_dual in pi2; eassumption.
-- apply ll2llfrag in pi1; assumption.
+- cbn in pi2. rewrite <- ll2ll_dual in pi2. eassumption.
+- assumption.
 Qed.
 
 End Atoms.
