yalla/mell_Prop.v
@@ -21,12 +21,9 @@ Context {atom : DecType}.
 (** ** 1. define formulas *)
 
 Inductive formula :=
-| var : atom -> formula
-| covar : atom -> formula
-| tens : formula -> formula -> formula
-| parr : formula -> formula -> formula
-| oc : formula -> formula
-| wn : formula -> formula.
+| var (_ : atom) | covar (_ : atom)
+| tens (_ _ : formula) | parr (_ _ : formula)
+| oc (_ : formula) | wn (_ : formula).
 
 Fixpoint dual A :=
 match A with
@@ -53,12 +50,12 @@ end.
 
 Lemma mell2ll_inj : injective mell2ll.
 Proof.
-intros A; induction A; intros B Heq; destruct B; inversion Heq ;
+intros A. induction A; intros B Heq; destruct B; inversion Heq ;
   try apply IHA in H0; try apply IHA1 in H0; try apply IHA2 in H1; subst; reflexivity.
 Qed.
 
 Lemma mell2ll_dual A : formulas.dual (mell2ll A) = mell2ll (dual A).
-Proof. induction A; cbn;rewrite ? IHA, ? IHA1 ,? IHA2; reflexivity. Qed.
+Proof. induction A; cbn; rewrite ? IHA, ? IHA1 ,? IHA2; reflexivity. Qed.
 
 Lemma mell2ll_map_wn l : map mell2ll (map wn l) = map formulas.wn (map mell2ll l).
 Proof. induction l as [ | a l IHl]; [ | cbn; rewrite IHl ]; reflexivity. Qed.
@@ -66,10 +63,10 @@ Proof. induction l as [ | a l IHl]; [ | cbn; rewrite IHl ]; reflexivity. Qed.
 Lemma mell2ll_map_wn_inv l1 l2 : map formulas.wn l1 = map mell2ll l2 ->
   exists l2', l2 = map wn l2' /\ l1 = map mell2ll l2'.
 Proof.
-induction l1 in l2 |- *; intros Heq; destruct l2; inversion Heq.
+induction l1 as [|a l1 IHl1] in l2 |- *; intros Heq; destruct l2; inversion Heq.
 - exists nil; split; reflexivity.
 - apply IHl1 in H1.
-  destruct f; inversion H0; subst.
+  destruct f; inversion H0. subst.
   destruct H1 as (l2' & -> & ->).
   exists (f :: l2'); split; reflexivity.
 Qed.
@@ -78,30 +75,17 @@ Qed.
 (** ** 3. define proofs *)
 
 Inductive mell : list formula -> Prop :=
-| ax_r : forall X, mell (covar X :: var X :: nil)
-| ex_r : forall l1 l2, mell l1 ->
-              Permutation l1 l2 -> mell l2
-| tens_r : forall A B l1 l2,
-              mell (A :: l1) -> mell (B :: l2) ->
-              mell (tens A B :: l1 ++ l2)
-| parr_r : forall A B l,
-              mell (A :: B :: l) ->
-              mell (parr A B :: l)
-| oc_r : forall A l,
-              mell (A :: map wn l) ->
-              mell (oc A :: map wn l)
-| de_r : forall A l,
-              mell (A :: l) ->
-              mell (wn A :: l)
-| wk_r : forall A l,
-              mell l ->
-              mell (wn A :: l)
-| co_r : forall A l,
-              mell (wn A :: wn A :: l) ->
-              mell (wn A :: l).
+| ax_r X : mell (covar X :: var X :: nil)
+| ex_r l1 l2 : mell l1 -> Permutation l1 l2 -> mell l2
+| tens_r A B l1 l2 : mell (A :: l1) -> mell (B :: l2) -> mell (tens A B :: l1 ++ l2)
+| parr_r A B l : mell (A :: B :: l) -> mell (parr A B :: l)
+| oc_r A l : mell (A :: map wn l) -> mell (oc A :: map wn l)
+| de_r A l : mell (A :: l) -> mell (wn A :: l)
+| wk_r A l : mell l -> mell (wn A :: l)
+| co_r A l : mell (wn A :: wn A :: l) -> mell (wn A :: l).
 
 Instance mell_perm : Proper ((@Permutation _) ==> Basics.impl) mell.
-Proof. intros l1 l2 HP pi; eapply ex_r; eassumption. Qed.
+Proof. intros l1 l2 HP pi. eapply ex_r; eassumption. Qed.
 
 
 (** ** 4. characterize corresponding [ll] fragment *)
@@ -132,74 +116,66 @@ Definition pfrag_mell := @ll_def.mk_pfrag atom  ll_def.pcut_none ll_def.NoAxioms
 
 Lemma mell2mellfrag l : mell l -> inhabited (ll_def.ll pfrag_mell (map mell2ll l)).
 Proof.
-intros pi; induction pi; try (now ((try inversion IHpi); do 2 constructor)); rewrite ? map_app.
+intros pi. induction pi; try ((try inversion IHpi); do 2 constructor; assumption); rewrite ? map_app.
 - apply Permutation_Permutation_transp in H.
   induction H.
-  + inversion IHpi; constructor; assumption.
-  + inversion IHpi; constructor.
+  + inversion IHpi. constructor. assumption.
+  + inversion IHpi. constructor.
     eapply ll_def.ex_r; [ eassumption | ].
     apply Permutation_Type_map, Permutation_Type_app_head, Permutation_Type_swap.
   + apply IHPermutation_transp2.
     * apply Permutation_Permutation_transp in H.
       eapply ex_r; eassumption.
     * apply IHPermutation_transp1; assumption.
-- inversion IHpi1; inversion IHpi2; constructor.
+- inversion IHpi1. inversion IHpi2. constructor.
   eapply ll_def.ex_r.
   + apply (ll_def.tens_r X X0).
-  + cbn; rewrite map_app.
-    apply Permutation_Type_cons, Permutation_Type_app_comm; reflexivity.
-- inversion IHpi; constructor.
-  cbn; rewrite mell2ll_map_wn.
-  apply ll_def.oc_r.
-  rewrite <- mell2ll_map_wn; assumption.
+  + cbn. rewrite map_app.
+    apply Permutation_Type_cons, Permutation_Type_app_comm. reflexivity.
+- inversion IHpi. constructor.
+  cbn. rewrite mell2ll_map_wn. apply ll_def.oc_r. rewrite <- mell2ll_map_wn. assumption.
 Qed.
 
 Lemma mellfrag2mell l : ll_def.ll pfrag_mell (map mell2ll l) -> mell l.
 Proof.
 intros pi.
 remember (map mell2ll l) as l0.
-revert l Heql0; induction pi; intros l' Heql0; subst;
-  try now (destruct l'; inversion Heql0; destruct f; inversion H0).
-- symmetry in Heql0; decomp_map Heql0; subst.
-  destruct l1; inversion Heql4.
-  destruct x; inversion Heql2.
-  destruct x0; inversion Heql0; subst.
+revert l Heql0. induction pi; intros l' Heql0; subst;
+  try (destruct l'; inversion Heql0; destruct f; inversion H0; assumption).
+- symmetry in Heql0. decomp_map Heql0. subst.
+  destruct l1; inversion Heql4. destruct x; inversion Heql2. destruct x0; inversion Heql0. subst.
   apply ax_r.
 - cbn in p.
   apply Permutation_Type_map_inv in p
     as [l'' Heq HP%Permutation_Type_sym%Permutation_Type_Permutation].
   eapply ex_r; [ | eassumption ].
-  apply IHpi; assumption.
-- symmetry in Heql0; decomp_map Heql0; subst; symmetry in Heql0.
+  apply IHpi. assumption.
+- symmetry in Heql0. decomp_map Heql0. subst. symmetry in Heql0.
   destruct (mell2ll_map_wn_inv _ _ Heql0) as (l' & -> & ->).
   apply Permutation_Type_map_inv in p as [l'' ->].
-  apply (Permutation_Type_map wn), Permutation_Type_Permutation in p.
   eapply (@ex_r (l0 ++ map wn l'' ++ l5)).
-  + apply IHpi; list_simpl; rewrite mell2ll_map_wn; reflexivity.
-  + symmetry; apply Permutation_app_head, Permutation_app_tail; assumption.
-- symmetry in Heql0; decomp_map Heql0; subst.
-  destruct x; inversion Heql2; subst.
+  + apply IHpi. list_simpl. rewrite mell2ll_map_wn. reflexivity.
+  + symmetry. apply Permutation_app_head, Permutation_app_tail, Permutation_map, Permutation_Type_Permutation, p.
+- discriminate f.
+- symmetry in Heql0. decomp_map Heql0. subst.
+  destruct x; inversion Heql2. subst.
   eapply ex_r; [ apply tens_r | ].
-  + apply IHpi1; reflexivity.
-  + apply IHpi2; reflexivity.
-  + apply Permutation_cons, Permutation_app_comm; reflexivity.
-- destruct l'; inversion Heql0.
-  destruct f; inversion H0; subst.
-  apply parr_r, IHpi; reflexivity.
-- destruct l'; inversion Heql0.
-  destruct f; inversion H0; subst.
+  + apply IHpi1. reflexivity.
+  + apply IHpi2. reflexivity.
+  + apply Permutation_cons, Permutation_app_comm. reflexivity.
+- destruct l'; inversion Heql0. destruct f; inversion H0. subst.
+  apply parr_r, IHpi. reflexivity.
+- destruct l'; inversion Heql0. destruct f; inversion H0. subst.
   apply mell2ll_map_wn_inv in H1 as (l'' & -> & ->).
-  apply oc_r, IHpi; cbn; rewrite mell2ll_map_wn; reflexivity.
-- destruct l'; inversion Heql0.
-  destruct f; inversion H0; subst.
-  apply de_r, IHpi; reflexivity.
-- destruct l'; inversion Heql0.
-  destruct f; inversion H0; subst.
-  apply wk_r, IHpi; reflexivity.
-- symmetry in Heql0; decomp_map Heql0; subst.
-  destruct x; inversion Heql2; subst.
-  apply co_r, IHpi; reflexivity.
-- inversion f.
+  apply oc_r, IHpi. cbn. rewrite mell2ll_map_wn. reflexivity.
+- destruct l'; inversion Heql0. destruct f; inversion H0. subst.
+  apply de_r, IHpi. reflexivity.
+- destruct l'; inversion Heql0. destruct f; inversion H0. subst.
+  apply wk_r, IHpi. reflexivity.
+- symmetry in Heql0; decomp_map Heql0. subst.
+  destruct x; inversion Heql2. subst.
+  apply co_r, IHpi. reflexivity.
+- discriminate f.
 - destruct a.
 Qed.
 
@@ -207,7 +183,7 @@ Lemma inhmellfrag2mell l : inhabited (ll_def.ll pfrag_mell (map mell2ll l)) -> m
 Proof.
 assert (inhabited (ll_def.ll pfrag_mell (map mell2ll l)) -> inhabited (mell l)) as Hi
   by apply inhabited_covariant, mellfrag2mell.
-intros H%Hi; destruct H; assumption.
+intros [H]%Hi. assumption.
 Qed.
 
 
@@ -217,8 +193,7 @@ Qed.
 
 Lemma ax_gen_r A : mell (dual A :: A :: nil).
 Proof.
-apply mellfrag2mell.
-cbn; rewrite <- mell2ll_dual.
+apply mellfrag2mell. cbn. rewrite <- mell2ll_dual.
 eapply ll_def.ex_r; [ apply ll_def.ax_exp | apply Permutation_Type_swap ].
 Qed.
 
@@ -226,11 +201,10 @@ Qed.
 
 Lemma cut_r A l1 l2 : mell (A :: l1) -> mell (dual A :: l2) -> mell (l1 ++ l2).
 Proof.
-intros pi1%mell2mellfrag pi2%mell2mellfrag.
-apply inhmellfrag2mell.
-destruct pi1 as [ pi1 ]; destruct pi2 as [ pi2 ]; constructor.
+intros [pi1]%mell2mellfrag [pi2]%mell2mellfrag.
+apply inhmellfrag2mell. constructor.
 rewrite map_app.
-eapply ll_cut.cut_r_axfree; [ intros a; destruct a | rewrite mell2ll_dual | ]; eassumption.
+eapply ll_cut.cut_r_axfree; [ intros [] | rewrite mell2ll_dual | ]; eassumption.
 Qed.
 
 End Atoms.
