yalla/subs.v
@@ -3,8 +3,7 @@
 
 (** * Substitutions in Linear Logic formulas and proofs *)
 
-From OLlibs Require Import infinite List_more Permutation_Type GPermutation_Type
-                           Dependent_Forall_Type.
+From OLlibs Require Import infinite List_more Permutation_Type GPermutation_Type Dependent_Forall_Type.
 From Yalla Require Export ll_def.
 
 Set Implicit Arguments.
@@ -13,6 +12,7 @@ Set Implicit Arguments.
 Section Atoms.
 
 Context {atom : DecType}.
+Notation formula := (@formula atom).
 
 Definition ateq := @eqb atom.
 Definition ateq_eq := @eqb_eq atom.
@@ -23,18 +23,13 @@ Definition ateq_eq := @eqb_eq atom.
 Definition repl_at x y A := if ateq x y then A else var x.
 
 Lemma repl_at_eq x y A : x = y -> repl_at x y A = A.
-Proof.
-intros ->; unfold repl_at.
-rewrite (proj2 (ateq_eq _ _) (eq_refl _)); reflexivity.
-Qed.
+Proof. intros ->. unfold repl_at. rewrite (proj2 (ateq_eq _ _) (eq_refl _)). reflexivity. Qed.
 
 Lemma repl_at_neq x y A : x <> y -> repl_at x y A = var x.
 Proof.
-intros Hneq; unfold repl_at.
-case_eq (ateq x y); intros Heqb; [ | reflexivity ].
-exfalso.
-rewrite ateq_eq in Heqb.
-contradiction Heqb.
+intros Hneq. unfold repl_at.
+destruct (ateq x y) eqn:Heqb; [ | reflexivity ].
+exfalso. rewrite ateq_eq in Heqb. contradiction Heqb.
 Qed.
 
 (** Substitution in [formula]: substitutes [x] by [C] in [A] *)
@@ -54,16 +49,107 @@ match A with
 | wn A      => wn (subs C x A)
 end.
 
-Lemma subs_dual A C x : subs C x (dual A) = dual (subs C x A).
+Lemma subs_refl x A : subs (var x) x A = A.
 Proof.
-induction A; cbn; rewrite ? bidual;
-  try (now rewrite IHA); try (now rewrite IHA1, IHA2); reflexivity.
+induction A as [ a | a | | | | | | | | | | ]; cbn; rewrite ?IHA, ?IHA1, ?IHA2; try reflexivity.
+- destruct (eq_dt_dec a x) eqn:Heq.
+  + rewrite repl_at_eq by assumption. subst. reflexivity.
+  + rewrite repl_at_neq by assumption. reflexivity.
+- destruct (eq_dt_dec a x) eqn:Heq.
+  + rewrite repl_at_eq by assumption. subst. reflexivity.
+  + rewrite repl_at_neq by assumption. reflexivity.
 Qed.
+
+Lemma subs_dual A C x : subs C x (dual A) = dual (subs C x A).
+Proof. induction A; cbn; rewrite ? bidual, ? IHA, ? IHA1, ? IHA2; reflexivity. Qed.
+
+(** Parallel substitution in [formula] with distinguished substitution for positive and negative atoms *)
+Fixpoint psubs2 (sl sr : atom -> formula) (A : formula) :=
+match A with
+| var x     => sl x
+| covar x   => dual (sr x)
+| one       => one
+| bot       => bot
+| tens A B  => tens (psubs2 sl sr A) (psubs2 sl sr B)
+| parr A B  => parr (psubs2 sl sr A) (psubs2 sl sr B)
+| zero      => zero
+| top       => top
+| aplus A B => aplus (psubs2 sl sr A) (psubs2 sl sr B)
+| awith A B => awith (psubs2 sl sr A) (psubs2 sl sr B)
+| oc A      => oc (psubs2 sl sr A)
+| wn A      => wn (psubs2 sl sr A)
+end.
+
+Lemma dual_psubs2 sl sr A : dual (psubs2 sl sr A) = psubs2 sr sl (dual A).
+Proof. induction A; cbn; rewrite ? IHA, ? IHA1, ? IHA2, ?bidual; reflexivity. Qed.
+
+Lemma psubs2_var A : psubs2 var var A = A.
+Proof. induction A; cbn; rewrite ? IHA, ? IHA1, ? IHA2; reflexivity. Qed.
+
+Lemma psubs2_comp rl rr sl sr A :
+  psubs2 rl rr (psubs2 sl sr A) = psubs2 (fun x => psubs2 rl rr (sl x)) (fun x => psubs2 rr rl (sr x)) A.
+Proof. induction A; cbn; rewrite ? IHA, ? IHA1, ? IHA2, ? dual_psubs2; reflexivity. Qed.
+
+Lemma subs_psubs2 C x A : subs C x A = psubs2 (fun y => repl_at y x C) (fun y => repl_at y x C) A.
+Proof. induction A; cbn; rewrite ? IHA, ? IHA1, ? IHA2; reflexivity. Qed.
+
+
+(** Monotony of connectives *)
+
+(* With restriction to occurring atoms *)
+Lemma psubs2_monot_loc P A sl sr :
+  Forall_inf (fun x => ll P (sl x :: dual (sr x) :: nil)) (atom_list A) ->
+  ll P (psubs2 sl sr A :: psubs2 sl sr (dual A) :: nil).
+Proof.
+induction A; cbn; intros Hfv.
+- inversion Hfv. assumption.
+- ll_swap. inversion Hfv. assumption.
+- ll_swap. apply bot_r, one_r.
+- apply bot_r, one_r.
+- ll_swap. apply parr_r.
+  cons2app. eapply ex_r; [ | apply PCPermutation_Type_app_rot ].
+  rewrite app_assoc. apply tens_r.
+  + apply Forall_inf_app_l in Hfv.
+    apply IHA1. assumption.
+  + apply Forall_inf_app_r in Hfv.
+    apply IHA2. assumption.
+- apply parr_r.
+  cons2app. eapply ex_r; [ | apply PCPermutation_Type_app_rot ].
+  rewrite app_assoc. apply tens_r.
+  + apply Forall_inf_app_r in Hfv.
+    specialize (IHA2 Hfv). ll_swap in IHA2. assumption.
+  + apply Forall_inf_app_l in Hfv.
+    specialize (IHA1 Hfv). ll_swap in IHA1. assumption.
+- ll_swap. apply top_r.
+- apply top_r.
+- eapply plus_r1 in IHA1; [ | eapply Forall_inf_app_l, Hfv ]. ll_swap in IHA1.
+  eapply plus_r2 in IHA2; [ | eapply Forall_inf_app_r, Hfv ]. ll_swap in IHA2.
+  ll_swap. apply with_r; eassumption.
+- apply with_r; ll_swap; [ apply plus_r1 | apply plus_r2 ]; ll_swap.
+  + eapply IHA1, Forall_inf_app_l, Hfv.
+  + eapply IHA2, Forall_inf_app_r, Hfv.
+- change (ll P (oc (psubs2 sl sr A) :: map wn (psubs2 sl sr (dual A) :: nil))).
+  apply oc_r.
+  specialize (IHA Hfv). ll_swap in IHA.
+  cbn. ll_swap. apply de_r. assumption.
+- apply de_r in IHA; [ | assumption ]. ll_swap in IHA.
+  ll_swap.
+  change (ll P (oc (psubs2 sl sr (dual A)) :: map wn (psubs2 sl sr A :: nil))).
+  apply oc_r. assumption.
+Qed.
+
+Lemma psubs2_monot P sl sr (Hs : forall x, ll P (sl x :: dual (sr x) :: nil)) A :
+  ll P (psubs2 sl sr A :: psubs2 sl sr (dual A) :: nil).
+Proof. apply psubs2_monot_loc, forall_Forall_inf. intros ? _. apply Hs. Qed.
+
+Lemma ax_exp_from_monot P (A : formula) : ll P (A :: dual A :: nil).
+Proof. rewrite <- (psubs2_var A), dual_psubs2. apply psubs2_monot. intro. ll_swap. apply ax_r. Qed.
+
 
 (** Substitution in proofs *)
 
 Lemma subs_ll P A x l :
-  (forall C, pcut P C = true -> pcut P (subs A x C) = true) ->
+  (forall C, Bool.le (pcut P C) (pcut P (subs A x C))) ->
   ll P l ->
     ll (axupd_pfrag P (existT (fun x => x -> list formula) _
                             (fun a => map (subs A x) (projT2 (pgax P) a))))
@@ -72,68 +158,46 @@ Proof.
 intros Hcut pi.
 assert (forall l, map (subs A x) (map wn l) = map wn (map (subs A x) l)) as Hmapwn
   by (clear; induction l; [ | cbn; rewrite IHl ]; reflexivity).
-induction pi using ll_nested_ind; list_simpl; try (now constructor).
+induction pi using ll_nested_ind; list_simpl; try (constructor; assumption).
 - eapply ex_r; [ apply ax_exp | apply PCPermutation_Type_swap ].
 - eapply PCPermutation_Type_map in p.
   eapply ex_r; eassumption.
-- rewrite ? map_app, Hmapwn in IHpi; rewrite Hmapwn.
+- rewrite ? map_app, Hmapwn in IHpi. rewrite Hmapwn.
   eapply Permutation_Type_map in p.
   eapply ex_wn_r; eassumption.
-- rewrite concat_map.
-  apply mix_r.
-  + cbn; rewrite map_length; assumption.
+- rewrite concat_map. apply mix_r.
+  + cbn. rewrite map_length. assumption.
   + apply forall_Forall_inf.
     intros l' Hin.
     destruct (in_inf_map_inv (map (subs A x)) L l' Hin) as [l0 <- Hin'].
     apply (In_Forall_inf_in _ PL) in Hin' as [pi' Hin'].
     refine (Dependent_Forall_inf_forall_formula _ _ X Hin').
 - specialize Hmapwn with l.
-  rewrite Hmapwn.
-  apply oc_r.
-  rewrite <- Hmapwn; assumption.
-- refine (cut_r (subs A x A0) _ _ _); [ cbn; apply Hcut | rewrite <- subs_dual | ]; assumption.
-- apply (@gax_r _ (axupd_pfrag P (existT (fun x => x -> list formula) _
-                               (fun a => map (subs A x) (projT2 (pgax P) a)))) a).
+  rewrite Hmapwn. apply oc_r. rewrite <- Hmapwn. assumption.
+- refine (cut_r (subs A x A0) _ _ _); [ | rewrite <- subs_dual; assumption | assumption ].
+  specialize (Hcut A0).
+  eapply Bool.implb_true_iff, f. apply Bool.le_implb, Hcut.
+- apply (@gax_r _ (axupd_pfrag P (existT (fun x => x -> _) _
+                                         (fun a => map (subs A x) (projT2 (pgax P) a)))) a).
 Qed.
 
-Lemma subs_ll_axfree P : (projT1 (pgax P) -> False) -> forall A x l,
-  (forall C, pcut P C = true -> pcut P (subs A x C) = true) ->
+Lemma subs_ll_axfree P (P_axfree : notT (projT1 (pgax P))) A x l : (forall C, Bool.le (pcut P C) (pcut P (subs A x C))) ->
   ll P l -> ll P (map (subs A x) l).
 Proof.
-intros P_axfree A x l Hcut pi.
+intros Hcut pi.
 apply (subs_ll A x) in pi; [ | assumption ].
 eapply stronger_pfrag; [ | eassumption ].
-repeat split; try reflexivity.
-cbn; intros a.
-contradiction P_axfree.
+repeat split; try reflexivity. intro. contradiction P_axfree.
 Qed.
-
-
-(** ** Fresh atoms and associated properties *)
-
-Fixpoint atom_list A : list atom :=
-match A with
-| var x     => x :: nil
-| covar x   => x :: nil
-| one       => nil
-| bot       => nil
-| tens B C  => atom_list B ++ atom_list C
-| parr B C  => atom_list B ++ atom_list C
-| zero      => nil
-| top       => nil
-| aplus B C => atom_list B ++ atom_list C
-| awith B C => atom_list B ++ atom_list C
-| oc B      => atom_list B
-| wn B      => atom_list B
-end.
 
 End Atoms.
 
 
+(** ** Fresh atoms and associated properties *)
+
 Section InfAtoms.
 
 Context {atom : InfDecType}.
-
 Notation formula := (@formula atom).
 
 (** Provide an [Atom] which is fresh for [A] *)
@@ -146,26 +210,25 @@ induction A; cbn; intros Hincl;
   rewrite ? IHA, ? IHA1, ? IHA2;
   cbn; trivial;
   try now apply incl_app_inv in Hincl.
-  all: rewrite repl_at_neq; [ reflexivity | intros -> ].
-  all: apply (fresh_prop lat), (Hincl (fresh lat)).
-  all: left; reflexivity.
+all: rewrite repl_at_neq; [ reflexivity | intros -> ].
+all: apply (fresh_prop lat), (Hincl (fresh lat)).
+all: left; reflexivity.
 Qed.
 
 Lemma subs_fresh C A : subs C (fresh_of A) A = A.
-Proof. now intros; apply subs_fresh_incl. Qed.
+Proof. apply subs_fresh_incl. intro. exact id. Qed.
 
 (** Provide an [Atom] which is fresh for all elements of [l] *)
 Definition fresh_of_list (l : list formula) := fresh (flat_map atom_list l).
 
-Lemma subs_fresh_list_incl C lat (l : list formula) :
-  incl (flat_map atom_list l) lat -> map (subs C (fresh lat)) l = l.
+Lemma subs_fresh_list_incl C lat (l : list formula) : incl (flat_map atom_list l) lat -> map (subs C (fresh lat)) l = l.
 Proof.
-induction l; cbn; intros Hincl; [ reflexivity | ].
+induction l as [|a l IHl]; cbn; intros Hincl; [ reflexivity | ].
 apply incl_app_inv in Hincl.
 now rewrite subs_fresh_incl; [ rewrite IHl | ].
 Qed.
 
 Lemma subs_fresh_list C l : map (subs C (fresh_of_list l)) l = l.
-Proof. now intros; apply subs_fresh_list_incl. Qed.
+Proof. apply subs_fresh_list_incl. intro. exact id. Qed.
 
 End InfAtoms.
